Lemma/List/LengthInsertIdxEraseIdx/eq/Length/of/Lt_Length.lean
@@ -1,0 +1,27 @@
+import Lemma.List.LengthInsertIdx.eq.Add1Length.of.Le_Length
+import Lemma.Algebra.Le_Sub_1.of.Lt
+import Lemma.List.LengthEraseIdx.eq.SubLength_1.of.Lt_Length
+import Lemma.Algebra.EqAdd_Sub.of.Ge
+import Lemma.Algebra.Ge_1.of.Gt
+open List Algebra
+
+
+@[main]
+private lemma main
+  {dim : ℕ}
+  {s : List α}
+-- given
+  (h : dim < s.length)
+  (a : α) :
+-- imply
+  ((s.eraseIdx dim).insertIdx dim a).length = s.length := by
+-- proof
+  rw [LengthInsertIdx.eq.Add1Length.of.Le_Length] <;>
+    rw [LengthEraseIdx.eq.SubLength_1.of.Lt_Length h]
+  ·
+    apply (EqAdd_Sub.of.Ge ∘ Ge_1.of.Gt) h
+  ·
+    apply Le_Sub_1.of.Lt h
+
+
+-- created on 2025-10-04
