Lemma/List/Lt_LengthInsertIdxEraseIdx/of/Lt_Length.lean
@@ -1,0 +1,18 @@
+import Lemma.List.LengthInsertIdxEraseIdx.eq.Length.of.Lt_Length
+open List
+
+
+@[main]
+private lemma main
+  {dim : ℕ}
+  {s : List α}
+-- given
+  (h : dim < s.length)
+  (a : α) :
+-- imply
+  dim < ((s.eraseIdx dim).insertIdx dim a).length := by
+-- proof
+  rwa [LengthInsertIdxEraseIdx.eq.Length.of.Lt_Length h]
+
+
+-- created on 2025-10-04
