Lemma/Tensor/SumKeepdim/as/RepeatUnsqueezeSum.lean
@@ -1,9 +1,9 @@
 import stdlib.SEq
 import sympy.tensor.functions
-import Lemma.List.LengthInsertIdx.eq.Add1Length.of.Le_Length
-import Lemma.Algebra.Le_Sub_1.of.Lt
-import Lemma.Algebra.EqAdd_Sub.of.Lt
-open List Algebra
+import Lemma.Logic.SEq.of.EqCast.Eq
+import Lemma.List.Lt_LengthInsertIdxEraseIdx.of.Lt_Length
+import Lemma.List.EqSetInsertIdxEraseIdx.of.Lt_Length
+open Logic List
 
 
 @[main]
@@ -12,19 +12,17 @@ private lemma main
   {dim : ℕ}
 -- given
   (X : Tensor α s)
-  (h_dim : dim < s.length) :
+  (h : dim < s.length) :
 -- imply
-  have h_dim : dim < ((s.eraseIdx dim).insertIdx dim 1).length := by
-    rw [List.LengthInsertIdx.eq.Add1Length.of.Le_Length] <;>
-      rw [LengthEraseIdx.eq.SubLength_1.of.Lt_Length h_dim]
-    .
-      rwa [EqAdd_Sub.of.Ge]
-      apply Algebra.Ge_1.of.Gt h_dim
-    .
-      apply Le_Sub_1.of.Lt h_dim
-  X.sum_keepdim dim ≃ ((X.sum dim).unsqueeze dim).repeat s[dim] ⟨dim, h_dim⟩ := by
+  X.sum_keepdim dim ≃ ((X.sum dim).unsqueeze dim).repeat s[dim] ⟨dim, Lt_LengthInsertIdxEraseIdx.of.Lt_Length h 1⟩ := by
 -- proof
-  sorry
+  apply SEq.of.EqCast.Eq
+  · 
+    unfold Tensor.sum_keepdim
+    simp [h]
+  · 
+    simp [EqSetInsertIdxEraseIdx.of.Lt_Length h]
 
 
 -- created on 2025-10-03
+-- updated on 2025-10-04
